order-book/verify/Properties/OrderV2.lean
@@ -5,8 +5,10 @@ namespace Properties.OrderV2
 
 open PlutusCore.UPLC.Term (Program)
 open PlutusCore.Data (Data)
-open CardanoLedgerApi.V3 (Redeemer)
-open Properties.Soundness (spend_sound_theorem)
+open PlutusCore.ByteString (ByteString)
+open CardanoLedgerApi.IsData.Class (IsData)
+open CardanoLedgerApi.V3 (Redeemer TxOutRef)
+open Properties.Soundness (OrderDatum spend_sound_theorem)
 
 set_option warn.sorry false
 
@@ -14,10 +16,24 @@ set_option warn.sorry false
 
 def orderV2Validator : Program := orderV2Script.script
 
+def tagData : Option TxOutRef → Data
+  | none     => Data.Constr 1 []
+  | some ref => Data.Constr 0 [IsData.toData ref]
+
+def orderData (tag : Option TxOutRef) (d : OrderDatum) : Data :=
+  Data.Constr 0
+  [ Data.B d.owner,
+    Data.I d.amount,
+    Data.B d.policyId,
+    Data.B d.assetName,
+    tagData tag ]
+
 theorem spend_sound :
   ∀ (redeemer : Redeemer),
+    -- (tag : Option TxOutRef),
   -- let redeemer : Redeemer := Data.Constr 0 [Data.I idx]
-  spend_sound_theorem orderV2Validator redeemer
+  let tag := none
+  spend_sound_theorem orderV2Validator redeemer (orderData tag)
   := by blaster
 
 end Properties.OrderV2
